Update Dutch_National_Flag_Monad.thy
Added and proved some lemmators of add_high and inc_index. This is commit before clean up

Monad_Play Around/DNFP/Dutch_National_Flag_Monad.thy
@@ -7,7 +7,7 @@ begin
 
 text\<open>Monad definitions to encode and extract data from the monad\<close>
 datatype color = red | white | blue
-
+section\<open>Monad definitions\<close>
 record env = 
   high :: "nat"
   low  :: "nat"
@@ -17,14 +17,11 @@ record env =
 definition return:: "'a \<Rightarrow> ('b, 'a) state" where "return = State_Monad.return"
 definition get:: "(env, env) state" where "get = State (\<lambda>x. (x,x))"
 definition put:: "env \<Rightarrow> (env, unit) state" where "put x = State (\<lambda>_. ((),x))"
-text\<open>Ask Stefan about how to do generic get\<close>
-definition get_gen:: "char list\<Rightarrow> (env, 'a) state" where "get_gen acc = do { x \<leftarrow> get; return (acc  x)}"
-
+definition get_gen:: "(env \<Rightarrow> 'b) \<Rightarrow> (env, 'b) state" where "get_gen acc = do { x \<leftarrow> get; return (acc  x)}"
 definition get_high:: "(env, nat) state" where "get_high = do { x \<leftarrow> get; return (high  x) }" 
 definition get_low:: "(env, nat) state" where "get_low = do { x \<leftarrow> get; return (low x) }" 
 definition get_i:: "(env, nat) state" where "get_i = do { x \<leftarrow> get; return (i x) }" 
 definition get_xs:: "(env, nat list) state" where "get_xs = do { x \<leftarrow> get; return (xs x) }" 
-
 definition set_high:: "env \<Rightarrow> nat \<Rightarrow> env" where "set_high v x =  
 \<lparr>            high = x,
              low = low v,
@@ -35,13 +32,11 @@ definition set_low:: "env \<Rightarrow> nat \<Rightarrow> env" where "set_low v 
              low = x,
              i = i v,
              xs = xs v \<rparr>"
-
 definition set_i:: "env \<Rightarrow> nat \<Rightarrow> env" where "set_i v x =  
 \<lparr>            high = high v,
              low = low v,
              i = x,
              xs = xs v \<rparr>"
-
 definition set_xs:: "env \<Rightarrow> nat list \<Rightarrow> env" where "set_xs v x =
 \<lparr>            high = high v,
              low = low v,
@@ -54,8 +49,11 @@ definition put_i:: "nat \<Rightarrow> (env, unit) state" where "put_i x = do { v
 definition put_xs:: "nat list \<Rightarrow> (env, unit) state" where "put_xs x = do { v \<leftarrow> get; put (set_xs v x) }"
 definition skip:: "(env, unit) state" where "skip = State (\<lambda>x. ((),x))"
 
+section\<open>DNFP\<close>
 
-definition swap:: "'a list \<Rightarrow> nat \<Rightarrow> nat \<Rightarrow> 'a list" where
+type_synonym 'a array = "'a list"
+
+definition swap:: "'a array \<Rightarrow> nat \<Rightarrow> nat \<Rightarrow> 'a array" where
 "swap l x y \<equiv> (if x < length l \<and> y < length l then l[x := l!y, y := l!x] else l)"
 
 lemma length_swap: "length(swap l x y) = length l"
@@ -83,16 +81,25 @@ definition inc_lowbound where
                   put_low (Suc l)
                 }"
 
+definition add_high where
+"add_high s j h \<equiv> do{
+                    put_xs (swap s j h)
+                  }"
+
 definition dec_highbound where
-"dec_highbound s j h\<equiv> do{
+"dec_highbound s j h \<equiv> do{
                     put_high (h - 1);
-                    put_xs (swap s j (h-1))
+                    add_high s j (h-1)
                 }"
 
 definition inc_index where
 "inc_index j \<equiv> do{
                   put_i (Suc j)
                 }"
+(*
+definition hoare_def where
+"hoare_def pre prog post \<equiv> "
+*)
 
 definition loop_update_action where
 "loop_update_action s j h \<equiv> 
@@ -137,7 +144,6 @@ value \<open>sorted(xs(snd(run_state (dnfp_mon 5) (init_env[0,2,2,1,2]))))\<clos
 value \<open>sorted(xs(snd(run_state (dnfp_mon 9) (init_env[0,2,2,0,1,0,2,1,2]))))\<close>
 value \<open>sorted(xs(snd(run_state (dnfp_mon 3) (init_env[2,1,0]))))\<close>
 
-
 section\<open>Definiton of all the Pre and postconditions\<close>
 
 subsection\<open>The invariants are taken from https://en.wikipedia.org/wiki/Dutch_national_flag_problem\<close>
@@ -145,7 +151,7 @@ definition low_invariant_is_0 where
 "low_invariant_is_0 arr l\<equiv> (\<forall>x. x < l \<longrightarrow> arr!x = 0)"
 
 definition invariant_low_to_j_is_1 where
-"invariant_low_to_j_is_1 arr l j \<equiv> (\<forall>x. x \<ge> l \<and> x < j \<longrightarrow> arr!x = 1)"
+"invariant_low_to_j_is_1 arr l j \<equiv> (\<forall>x. (x \<ge> l \<and> x < j) \<longrightarrow> arr!x = 1)"
 
 definition high_invariant_is_2 where
 "high_invariant_is_2 arr h\<equiv> (\<forall>x. x \<ge> h \<longrightarrow> arr!x = 2)"
@@ -155,13 +161,23 @@ definition invariants where
               \<and> invariant_low_to_j_is_1 arr l j
               \<and> high_invariant_is_2 arr h"
 
+definition invariants1 where
+"invariants1 arr l j h\<equiv> low_invariant_is_0 arr l
+              \<and> high_invariant_is_2 arr h"
+
 text\<open>This can be used in the other pre and post-conditions for the methods inside loop_update_actions\<close>
 
 text\<open>Should I just take the environment as a single parameter here?\<close>
+
+subsection\<open>Pre- and Postconditions\<close>
 definition loop_update_action_pre where
 "loop_update_action_pre l j n e \<equiv> length l \<ge> Suc n \<and> 
                                     high e > j \<and>
                                     invariants l (low e) j (high e)"
+
+definition loop_update_action_pre1 where
+"loop_update_action_pre1 e \<equiv> high e > j \<and>
+                             invariants1 l (low e) j (high e)"
 
 definition loop_update_action_post where
 "loop_update_action_post e e' \<equiv> length (xs e) = length (xs e')
@@ -185,6 +201,14 @@ definition inc_index_pre where
 "inc_index_pre l j e n \<equiv> loop_update_action_pre l j n e  
                               \<and> l!j = 1"
 
+definition add_high_pre where 
+"add_high_pre l j e n \<equiv> loop_update_action_pre l j n e  
+                              \<and> l!j > 1"
+
+definition inc_index_pre1 where 
+"inc_index_pre1 l j e n \<equiv> loop_update_action_pre1 l j n e  
+                              \<and> l!j = 1"
+
 definition inc_lowbound_post where 
 "inc_lowbound_post e e'\<equiv> high e = high e'
                           \<and> low e < low e'
@@ -198,51 +222,152 @@ definition dec_highbound_post where
                               \<and> i e = i e'
                               \<and> invariants (xs e') (low e') (i e') (high e')"
 
+definition add_high_post where 
+"add_high_post e e' \<equiv> high e = high e' 
+                       \<and> low e = low e'
+                       \<and> i e = i e'
+                       \<and> length (xs e) = length (xs e')
+                       \<and> invariants (xs e') (low e') (i e') (high e')"
+
 definition inc_index_post where 
 "inc_index_post e e' \<equiv> high e = high e' 
                        \<and> low e = low e'
                        \<and> i e < i e'
                        \<and> invariants (xs e') (low e') (i e') (high e')"
 
-lemma inc_lowbound_pre_dom:
-  assumes "inc_lowbound_pre l j e n"
-  shows "colored e \<subseteq> vertices" 
-        "x \<in> vertices - colored e"
-        "x \<notin> set (stack e)"
-  sorry
+definition inc_index_post1 where 
+"inc_index_post1 e e' \<equiv> high e = high e' 
+                       \<and> low e = low e'
+                       \<and> i e < i e'
+                       \<and> invariants1 (xs e') (low e') (i e') (high e')"
+
+section\<open>Simple pre- and post conditions\<close>
+
+
+definition dec_highbound_simple_pre where
+"dec_highbound_simple_pre l j h \<equiv> h < length l
+                                    \<and> j < h  
+                                    \<and> l!j > 1"
+definition dec_highbound_simple_post where 
+"dec_highbound_simple_post e e' \<equiv> length (xs e) > high e' 
+                              \<and> high e > high e' 
+                              \<and> low e = low e'
+                              \<and> i e = i e' 
+                              \<and> length (xs e) = length (xs e')"
+
+
+definition inc_lowbound_simple_pre where 
+"inc_lowbound_simple_pre l j h \<equiv> h < length l
+                                    \<and> j < h  
+                                    \<and> l!j < 1"
+
+definition inc_lowbound_simple_post where 
+"inc_lowbound_simple_post e e' \<equiv> length (xs e) > high e' 
+                              \<and> high e = high e' 
+                              \<and> low e < low e'
+                              \<and> i e < i e' 
+                              \<and> high e - i e > high e' - i e' 
+                              \<and> length (xs e) = length (xs e')"
+
+
+text\<open>This is a very simple precondition of index_j. It does not contain any invariants\<close>
+definition inc_index_simple_pre where
+"inc_index_simple_pre j h \<equiv> j < h"
+
+definition inc_index_post_simple where 
+"inc_index_post_simple e e' \<equiv> high e = high e' 
+                       \<and> low e = low e'
+                       \<and> i e < i e'
+                       \<and> high e - i e > high e' - i e' 
+                       \<and> xs e = xs e'"
+
+lemma inc_lowbound_simple: "\<lbrakk>inc_lowbound_simple_pre l j1 h \<and> l = xs e \<and> i e = j1 \<and> high e = h \<and> snd(run_state (inc_lowbound l j1) e) = e2\<rbrakk> \<Longrightarrow> inc_lowbound_simple_post e e2"
+  apply(simp_all add: inc_lowbound_simple_pre_def snd_def inc_lowbound_def get_low_def put_i_def put_xs_def set_xs_def put_low_def return_def get_def put_def set_low_def set_i_def inc_lowbound_simple_post_def)
+  apply(simp_all add: swap_def)
+  by (auto)
+
+lemma dec_highbound_simple: "\<lbrakk>dec_highbound_simple_pre l j1 h \<and> l = xs e \<and> i e = j1 \<and> high e = h \<and> snd(run_state (dec_highbound l j1 h) e) = e2\<rbrakk> \<Longrightarrow> dec_highbound_simple_post e e2"
+  apply(simp_all add: dec_highbound_simple_pre_def snd_def dec_highbound_def put_high_def put_xs_def put_def set_i_def dec_highbound_simple_post_def swap_def get_def)
+  apply(simp_all add: set_high_def set_xs_def add_high_def swap_def put_xs_def get_def put_def)
+  by (auto)
+
+text\<open>This goes through pretty easy\<close>
+lemma inc_index_j_simple: "\<lbrakk>inc_index_simple_pre j1 h \<and> i e = j1 \<and> high e = h \<and> snd(run_state (inc_index j1) e) = e2\<rbrakk> \<Longrightarrow> inc_index_post_simple e e2"
+  apply(simp_all add: inc_index_simple_pre_def snd_def inc_index_def put_i_def put_def set_i_def inc_index_post_simple_def get_def)
+  by (auto)
+
+lemma inv_aux: "\<lbrakk>xs e = xs e2; low e = low e2; i e < i e2; high e = high2; low_invariant_is_0 (xs e) (low e)\<rbrakk> \<Longrightarrow> low_invariant_is_0 (xs e2) (low e2)"
+  by(simp)
+
+text\<open>This is the same as above, but it contains the invariants that includes some universal quantifier\<close>
+lemma inc_index_j_simple_aux: "\<lbrakk>inc_index_simple_pre j1 h; i e = j1 ; high e = h; low_invariant_is_0 (xs e) (low e); 
+     high_invariant_is_2 (xs e) (high e); invariant_low_to_j_is_1 (xs e) (low e) (i e);
+     snd(run_state (inc_index j1) e) = e2 \<rbrakk> \<Longrightarrow> inc_index_post_simple e e2 \<Longrightarrow> low_invariant_is_0 (xs e2) (low e2) \<Longrightarrow> high_invariant_is_2 (xs e2) (high e2)"
+  by(simp_all add: inc_index_simple_pre_def snd_def inc_index_def put_i_def put_def set_i_def inc_index_post_simple_def get_def)
+
+lemma inc_index_j: "\<lbrakk>inc_index_pre1 l j e n; xs e = l; i e = j; snd(run_state (inc_index j) e) = e2\<rbrakk> \<Longrightarrow> inc_index_post1 e e2"
+  apply(simp_all add: snd_def  inc_index_def inc_index_post1_def inc_index_pre1_def loop_update_action_pre1_def)
+  apply(simp_all add: invariants1_def low_invariant_is_0_def high_invariant_is_2_def put_i_def get_def set_i_def put_def)
+  by (auto)
+
+text\<open>This is the proof of Inc Index that it preserves the invariants\<close>
+lemma inc_index_j_real: "\<lbrakk>inc_index_pre l j e n; xs e = l; i e = j; snd(run_state (inc_index j) e) = e2\<rbrakk> \<Longrightarrow> inc_index_post e e2"
+  apply(simp_all add: snd_def  inc_index_def inc_index_post_def inc_index_pre_def loop_update_action_pre_def)
+  apply(simp_all add: invariants_def low_invariant_is_0_def invariant_low_to_j_is_1_def high_invariant_is_2_def put_i_def get_def set_i_def put_def)
+  using less_Suc_eq by (force)
+
+lemma add_high_keep_invariants :"\<lbrakk>add_high_pre l j e n; xs e = l; l!j = 2; i e = j; high e = h; snd(run_state (add_high l j h) e) = e2\<rbrakk> \<Longrightarrow> add_high_post e e2"
+  apply(simp_all add: add_high_pre_def loop_update_action_pre_def invariants_def add_high_post_def add_high_def snd_def)
+  apply(simp_all add: put_xs_def put_def get_def set_xs_def swap_def)
+proof -
+assume a1: "Suc n \<le> length l \<and> j < h \<and> low_invariant_is_0 l (low e) \<and> invariant_low_to_j_is_1 l (low e) j \<and> high_invariant_is_2 l h"
+assume a2: "l ! j = 2"
+  assume a3: "\<lparr>high = h, low = low e, i = j, xs = if j < length l \<and> h < length l then l[j := l ! h, h := l ! j] else l\<rparr> = e2"
+  then have "(if j < length l \<and> h < length l then l[j := l ! h, h := 2] else l) = xs e2"
+    using a2 by fastforce
+  then show "h = high e2 \<and> low e = low e2 \<and> j = i e2 \<and> length l = length (xs e2) \<and> low_invariant_is_0 (xs e2) (low e2) \<and> invariant_low_to_j_is_1 (xs e2) (low e2) (i e2) \<and> high_invariant_is_2 (xs e2) (high e2)"
+    using a3 a2 a1 by (metis high_invariant_is_2_def le_refl list_update_id select_convs(1) select_convs(2) select_convs(3))
+qed
+
+lemma dec_highbound: "\<lbrakk>dec_highbound_pre l j e n; l = xs e;i e = j; l!j = 2;high e = h; h < length (xs e) ;snd(run_state (dec_highbound l j h) e) = e2\<rbrakk>
+                       \<Longrightarrow>  h = (Suc (high e2)) \<Longrightarrow> dec_highbound_post e e2"
+  apply(simp_all add: dec_highbound_pre_def snd_def dec_highbound_def loop_update_action_pre_def invariants_def dec_highbound_post_def)
+  apply(simp_all add: put_xs_def put_high_def get_def put_def set_xs_def swap_def set_high_def)
+  apply(simp_all add: low_invariant_is_0_def invariant_low_to_j_is_1_def high_invariant_is_2_def add_high_def)
+  apply(simp_all add: swap_def put_xs_def get_def put_def set_xs_def)
+  sledgehammer
 
 lemma inc_lowbound_post:
-"\<lbrakk>inc_lowbound_pre l j e n; snd (run_state (inc_lowbound l j) e) = e2\<rbrakk> \<Longrightarrow> inc_lowbound_post e e2"
+"\<lbrakk>inc_lowbound_pre l j e n; xs e = l; i e = j; snd (run_state (inc_lowbound l j) e) = e2\<rbrakk> \<Longrightarrow> inc_lowbound_post e e2"
   apply(simp_all add: inc_lowbound_pre_def loop_update_action_pre_def  get_low_def inc_lowbound_post_def)
-  apply(simp_all add: inc_lowbound_def invariants_def  invariant_low_to_j_is_1_def low_invariant_is_0_def high_invariant_is_2_def )
-  apply(simp_all add: swap_def get_low_def return_def get_def high_def put_xs_def low_def iso_tuple_fst_def tuple_iso_tuple_def fst_def repr_def iso_tuple_snd_def)
-  apply(simp_all add: put_def snd_def put_i_def get_def env_ext_Tuple_Iso_def set_i_def)
-  apply(induction l)
-   apply simp
-  sorry
+  apply(simp_all add: inc_lowbound_def invariants_def  invariant_low_to_j_is_1_def low_invariant_is_0_def high_invariant_is_2_def)
+  apply(simp_all add: swap_def get_low_def return_def get_def  put_xs_def fst_def snd_def)
+  apply(simp_all add: put_def snd_def put_i_def get_def set_i_def set_xs_def put_low_def set_low_def)
+  by(auto)
 
-lemma inc_lowbound_post:
-"\<lbrakk>init_env l = e; length l = Suc n; low e = l1; i e = j1; high e = h1; 
-    h1 > j1; l!j1 < 1 ; snd (run_state (inc_lowbound l j1) e) = e2; high e2 = h2; i e2 = j2\<rbrakk> \<Longrightarrow> (h2 - j2) \<le> (h1 - j1)"
+lemma inc_lowbound_post1:
+"\<lbrakk>inc_lowbound_pre l j1 e n; xs e = l; i e = j1; high e = h1;
+    h1 > j1; l!j1 < 1 ; snd (run_state (inc_lowbound l j1) e) = e2; high e2 = h2; i e2 = j2\<rbrakk> \<Longrightarrow> (h2 - j2) \<le> (h1 - j1) \<Longrightarrow> h2 = h1 \<Longrightarrow> j2 > j1"
   apply(simp_all add: snd_def inc_lowbound_def get_low_def return_def swap_def put_i_def put_def)
   apply(simp_all add: put_low_def set_i_def set_low_def get_def put_def put_xs_def set_xs_def)
-  apply(simp_all add: low_def Record.iso_tuple_snd_def Record.iso_tuple_fst_def fst_def env_ext_Tuple_Iso_def Record.tuple_iso_tuple_def snd_def)
-  apply(simp add: init_env_def low_def high_def Record.iso_tuple_fst_def fst_def Record.tuple_iso_tuple_def env_ext_Tuple_Iso_def)
-   apply(simp_all only: repr_def iso_tuple_snd_def low_def high_def Record.iso_tuple_fst_def fst_def Record.tuple_iso_tuple_def env_ext_Tuple_Iso_def)
-  apply(simp_all add: id_def)
-  sledgehammer
+  by (auto)
+
+lemma inc_lowbound_post2:
+"\<lbrakk>inc_lowbound_pre l j1 e n; xs e = l; i e = j1; high e = h1;
+    h1 > j1; l!j1 = 0 ; snd (run_state (inc_lowbound l j1) e) = e2\<rbrakk> \<Longrightarrow> high e = high e2 \<Longrightarrow>  j2 > j1  \<Longrightarrow> inc_lowbound_post e e2"
+  apply(simp_all add: snd_def inc_lowbound_def loop_update_action_pre_def  get_low_def return_def swap_def put_i_def put_def  inc_lowbound_pre_def inc_lowbound_post_def invariants_def)
+  apply(simp_all add:  low_invariant_is_0_def invariant_low_to_j_is_1_def high_invariant_is_2_def  put_low_def set_i_def set_low_def get_def put_def put_xs_def set_xs_def inc_lowbound_post1)
   sorry
 
 
 text\<open>The difference between high and i will never increase and will be decreased by loop_update_action\<close>
 lemma termination_loop_update_action:
-"\<lbrakk>init_env l = e; length l = Suc n; high e = h1; i e = j1; h1 > j1 ; snd (run_state (loop_update_action l j1 h1) e) = e2; high e2 = h2; i e2 = j2\<rbrakk> \<Longrightarrow> (h2 - j2) \<le> (h1 - j1)"
-  apply(simp_all add: snd_def high_def init_env_def i_def Record.iso_tuple_fst_def Record.tuple_iso_tuple_def fst_def Record.iso_tuple_snd_def)
-   apply(simp_all add: Record.repr_def env_ext_Tuple_Iso_def)
-  apply(simp_all add: loop_update_action_def inc_lowbound_def inc_lowbound_post dec_highbound_def put_i_def)
-   apply(simp only: loop_update_action_def inc_lowbound_def dec_highbound_def put_i_def)
-   apply(simp only: put_xs_def get_def get_low_def get_high_def put_def return_def put_low_def set_i_def set_xs_def put_high_def)
-  apply(simp only: set_low_def swap_def return_def set_high_def high_def low_def )
+"\<lbrakk>init_env l = e; high e = h1; i e = j1; h1 > j1 ; snd (run_state (loop_update_action l j1 h1) e) = e2; high e2 = h2; i e2 = j2\<rbrakk> \<Longrightarrow> (h2 - j2) \<le> (h1 - j1)"
+  apply(simp_all add: snd_def init_env_def loop_update_action_def)
+  apply(simp_all only: inc_lowbound_def dec_highbound_def inc_index_def)
+  apply(simp_all only: get_low_def put_xs_def get_def put_def put_i_def set_xs_def set_i_def put_low_def set_low_def put_high_def)
+  apply(simp_all only: swap_def set_high_def dec_highbound_simple inc_lowbound_simple inc_index_j_simple)
+  sledgehammer
   sorry
 
 
